lib/st2.fst
@@ -1,10 +1,46 @@
-module ST2
-assume val v0 : a:Type -> a -> Tot a
-assume val v1 : a:Type -> a -> Tot a
-
+module Comp
+open Heap
 type heap2 = heap * heap
-
 kind STWP (a:Type) = (a -> heap -> Type) -> heap -> Type
+kind PUREWP (a:Type) = (a -> Type) -> Type
+kind ALLPost (a:Type) = result a -> heap -> Type
+
+monad_lattice {
+  STATE2:: (* STATE a wp wlp *)
+          kind Pre     = heap2 -> Type
+          kind Post (a:Type) = a -> heap2 -> Type
+          kind WP (a:Type) = Post a -> Pre
+          type return   (a:Type) (x:a) (p:Post a) = p x
+          type bind_wp  (a:Type) (b:Type) (wp1:WP a) (wlp1:WP a) (wp2:(a -> WP b)) (wlp2:(a -> WP b)) (p:Post b) (h0:heap2) =
+              wp1 (fun a h1 -> wp2 a p h1) h0
+          type bind_wlp (a:Type) (b:Type) (wlp1:WP a) (wlp2:(a -> WP b)) (p:Post b) (h0:heap2) = wlp1 (fun a -> wlp2 a p) h0
+          type if_then_else (a:Type) (p:Type) (wp_then:WP a) (wp_else:WP a) (post:Post a) (h0:heap2) =
+              (if p
+               then wp_then post h0
+               else wp_else post h0)
+          type ite_wlp  (a:Type) (wlp_cases:WP a) (post:Post a) (h0:heap2) =
+              (forall (a:a) (h:heap2). wlp_cases (fun a1 h1 -> a=!=a1 \/ h=!=h1) h0 \/ post a h)
+          type ite_wp (a:Type) (wlp_cases:WP a) (wp_cases:WP a) (post:Post a) (h0:heap2) =
+              (forall (a:a) (h:heap2). wlp_cases (fun a1 h1 -> a=!=a1 \/ h=!=h1) h0 \/ post a h)
+              /\ wp_cases (fun a h_ -> True) h0
+          type wp_binop (a:Type) (wp1:WP a) ('op:Type -> Type -> Type) (wp2:WP a) (p:Post a) (h:heap2) =
+              'op (wp1 p h) (wp2 p h)
+          type wp_as_type (a:Type) (wp:WP a) = (forall (p:Post a) (h:heap2). wp p h)
+          type close_wp (a:Type) (b:Type) (wp:(b -> WP a)) (p:Post a) (h:heap2) = (forall (b:b). wp b p h)
+          type close_wp_t (a:Type) (wp:(Type -> WP a)) (p:Post a) (h:heap2) = (forall (b:Type). wp b p h)
+          type assert_p (a:Type) ('P:Type) (wp:WP a) (p:Post a) (h:heap2) = ('P /\ wp p h)
+          type assume_p (a:Type) ('P:Type) (wp:WP a) (p:Post a) (h:heap2) = ('P ==> wp p h)
+          type null_wp (a:Type) (p:Post a) (h:heap2) = (forall (x:a) (h':heap2). p x h')
+          type trivial (a:Type) (wp:WP a) = (forall h0. wp (fun r h1 -> True) h0)
+          with ST2 (a:Type) (pre:Pre) (post: (heap2 -> Post a)) =
+              STATE2 a
+                (fun (p:Post a) (h:heap2) -> pre h /\ (forall a h1. (pre h /\ post h a h1) ==> p a h1)) (* WP *)
+                (fun (p:Post a) (h:heap2) -> (forall a h1. (pre h /\ post h a h1) ==> p a h1))           (* WLP *)
+          and St2 (a:Type) = ST2 a (fun h -> True) (fun h0 r h1 -> True)
+  with
+  PURE   ~> STATE2 = (fun ('a:Type) ('wp:PUREWP 'a) ('p:STATE2.Post 'a) -> (fun h2 -> 'wp (fun a0 -> 'p a0 h2)));
+  STATE2 ~> ALL    = (fun ('a:Type) ('wp:STATE2.WP 'a) ('p:ALLPost 'a) -> (fun h -> False))
+}
 
 type comp (a:Type) (b:Type) (wp0:STWP a) (wp1:STWP b) (p:((a * b) -> heap2 -> Type)) (h2:heap2) =
     wp0 (fun y0 h0 ->
@@ -18,20 +54,24 @@ assume val compose2: a0:Type -> b0:Type -> wp0:(a0 -> STWP b0) -> wlp0:(a0 -> ST
                   -> =c1:(x1:a1 -> STATE b1 (wp1 x1) (wlp1 x1))
                   -> x0:a0
                   -> x1:a1
-                  -> ST2Core (b0 * b1)
+                  -> STATE2 (b0 * b1)
                              (comp b0 b1 (wp0 x0) (wp1 x1))
                              (comp b0 b1 (wlp0 x0) (wlp1 x1))
 
-module Sample
-open ST2
-open Heap
-
 let f x = x := !x - !x
 let g x = x := 0
-
 val equiv1: x:ref int
          -> y:ref int
-         -> ST2 (unit * unit)
-                (fun _ -> True) //x, y may be high-references
-                (fun _ _ h2' -> sel (fst h2') x == sel (snd h2') y) //their contents are equal afterwards
+         -> STATE2.ST2 (unit * unit)
+                (requires (fun _ -> True)) //x, y may be high-references
+                (ensures (fun _ _ h2' -> sel (fst h2') x == sel (snd h2') y)) //their contents are equal afterwards
 let equiv1 x y = compose2 f g x y
+
+
+let square x = x := !x * !x
+val equiv2: x:ref int
+         -> y:ref int
+         -> STATE2.ST2 (unit * unit)
+                (requires (fun h2 -> sel (fst h2) x = - (sel (snd h2) y)))     //x, y negatives of each other
+                (ensures (fun _ _ h2' -> sel (fst h2') x = sel (snd h2') y)) //their contents are equal afterwards
+let equiv2 x y = compose2 square square x y
